DeBruijnSSA/BinSyntax/Rewrite/Region/Compose/Structural/Basic.lean
@@ -13,9 +13,25 @@ def Eqv.packed {Γ : Ctx α ε} {R : LCtx α} (r : Eqv φ Γ R) : Eqv φ [(Γ.pa
 def Eqv.unpacked {Γ : Ctx α ε} {R : LCtx α} (r : Eqv φ [(Γ.pack, ⊥)] [R.pack]) (h : Γ.Pure)
   : Eqv φ Γ R := r.unpacked_out.unpacked_in h
 
--- TODO: (un)packed_in commutes with (un)packed_out
+theorem Eqv.unpacked_out_unpacked_in {Γ : Ctx α ε} {R : LCtx α}
+  {r : Eqv φ [(Γ.pack, ⊥)] [R.pack]} {h : Γ.Pure}
+  : (r.unpacked_in h).unpacked_out = r.unpacked_out.unpacked_in h := by
+  simp [unpacked_in, unpacked_out_let1]
+  induction r using Quotient.inductionOn
+  simp only [Term.Eqv.packE_def', vwk_id_quot, unpacked_out_quot, let1_quot]
+  rfl
 
--- TODO: packed_unpacked, unpacked_packed
+-- theorem Eqv.unpacked_out_packed_in {Γ : Ctx α ε} {R : LCtx α}
+--   {r : Eqv φ Γ [R.pack]} : r.packed_in.unpacked_out = r.unpacked_out.packed_in := sorry
+
+-- theorem Eqv.packed_out_unpacked_in {Γ : Ctx α ε} {R : LCtx α}
+--   {r : Eqv φ [(Γ.pack, ⊥)] R} {h : Γ.Pure}
+--   : (r.unpacked_in h).packed_out = r.packed_out.unpacked_in h := sorry
+
+-- theorem Eqv.packed_out_packed_in {Γ : Ctx α ε} {R : LCtx α}
+--   {r : Eqv φ Γ R} : r.packed_in.packed_out = r.packed_out.packed_in := sorry
+
+-- TODO: packed_unpacked, unpacked_packed via commutativity + cancellation
 
 -- TODO: {br, let1, let2, case, cfg}
 
